examples/miniML/hol2miniml/other-examples/example_parser_genScript.sml
@@ -1,30 +1,9 @@
 open HolKernel Parse boolLib bossLib; val _ = new_theory "example_parser_gen";
 
-open ml_translatorLib;
 open slr_parser_genTheory;
-open stringTheory listTheory;
+open ml_translatorTheory ml_translatorLib std_preludeTheory;
 
-
-val CHAR_def = Define `
-  CHAR (c:char) = NUM (ORD c)`;
-
-val _ = add_type_inv ``CHAR`` ``:num``
-
-val EqualityType_CHAR = prove(
-  ``EqualityType CHAR``,
-  EVAL_TAC THEN SRW_TAC [] [] THEN EVAL_TAC) |> store_eq_thm;
-
-val res = translate listTheory.HD;
-val res = translate listTheory.TL;
-val res = translate listTheory.LENGTH;
-val res = translate listTheory.MAP;
-val res = translate listTheory.APPEND;
-val res = translate listTheory.REV_DEF;
-val res = translate listTheory.REVERSE_REV;
-val res = translate pairTheory.FST;
-val res = translate pairTheory.SND;
-val res = translate combinTheory.o_DEF;
-val res = translate optionTheory.THE_DEF;
+val _ = translation_extends "std_prelude";
 
 val res = translate push_def;
 val res = translate pop_def;
@@ -46,6 +25,7 @@ val res = translate exitCond_def;
 val res = translate init_def;
 val res = translate doReduce_def;
 val res = translate parse_def;
+val res = translate (parser_def |> SIMP_RULE std_ss [mwhile_def]);
 
 val _ = export_theory();
 
